Remove use of modules

Core/Logic.v
@@ -9,300 +9,261 @@ From Coq Require Import
   Logic.FunctionalExtensionality
   Logic.PropExtensionality.
 
-Module Type OBJECT.
-  Parameter E F : ESig.
-  Parameter VF : Spec F.
-  Parameter VE : Spec E.
-End OBJECT.
+Definition Prec {E} VE F :=
+  @InterState E F VE ->
+  Trace (ThreadEvent F) ->
+  Prop.
 
-Module Predicates(O : OBJECT).
-  Import O.
+Definition Relt {E} VE F :=
+  @InterState E F VE -> Trace (ThreadEvent F) ->
+  @InterState E F VE -> Trace (ThreadEvent F) ->
+  Prop.
 
-  Definition Prec :=
-    @InterState E F VE ->
-    Trace (ThreadEvent F) ->
-    Prop.
+Definition PrecCompose {E VE F} (P : @Prec E VE F) (R : Relt VE F) : Prec VE F :=
+  fun t σ => exists s ρ, P s ρ /\ R s ρ t σ.
 
-  Definition Relt :=
-    @InterState E F VE -> Trace (ThreadEvent F) ->
-    @InterState E F VE -> Trace (ThreadEvent F) ->
-    Prop.
+Notation "R ;; G" := (PrecCompose R G) (left associativity, at level 38).
 
-  Definition rtp (R : Relt) : Prec :=
-    fun t σ => exists s ρ, R s ρ t σ.
+Definition ReltCompose {E VE F} (R G : @Relt E VE F) : Relt VE F :=
+  fun s ρ r τ => exists t σ, R s ρ t σ /\ G t σ r τ.
+Notation "R ; G" := (ReltCompose R G) (right associativity, at level 39).
 
-  Definition PrecCompose (P : Prec) (R : Relt) : Prec :=
-    fun t σ => exists s ρ, P s ρ /\ R s ρ t σ.
+Class HasImpl A :=
+  impl : A -> A -> A.
+Notation "P ==> Q" := (impl P Q) (right associativity, at level 41).
 
-  Notation "R ;; G" := (PrecCompose R G) (left associativity, at level 38).
+Global Instance implPrec E VE F : HasImpl (@Prec E VE F) :=
+  fun P Q s ρ => P s ρ -> Q s ρ.
 
-  Definition ReltCompose (R G : Relt) : Relt :=
-    fun s ρ r τ => exists t σ, R s ρ t σ /\ G t σ r τ.
-  Notation "R ; G" := (ReltCompose R G) (right associativity, at level 39).
+Global Instance implRelt E VE F : HasImpl (@Relt E VE F) :=
+  fun P Q s ρ t σ => P s ρ t σ -> Q s ρ t σ.
 
-  Class HasImpl A :=
-    impl : A -> A -> A.
-  Notation "P ==> Q" := (impl P Q) (right associativity, at level 41).
-  
-  Global Instance implPrec : HasImpl Prec :=
-    fun P Q s ρ => P s ρ -> Q s ρ.
-  
-  Global Instance implRelt : HasImpl Relt :=
-    fun P Q s ρ t σ => P s ρ t σ -> Q s ρ t σ.
-  
-  Class HasStable A :=
-    Stable : Relt -> A -> Prop.
-  
-  Global Instance stableRelt : HasStable Relt :=
-    fun R Q => forall s ρ t σ, (R; Q ==> Q) s ρ t σ /\ (Q; R ==> Q) s ρ t σ.
-  
-  Global Instance stablePrec : HasStable Prec :=
-    fun R P => forall s ρ, ((fun t σ => exists s ρ, P s ρ /\ R s ρ t σ) ==> P) s ρ.
+Class HasStable {E VE F} A :=
+  Stable : @Relt E VE F -> A -> Prop.
 
-  Class HasAll A :=
-    All : A -> Prop.
-  
-  Global Instance allRelt : HasAll Relt :=
-    fun R => forall s ρ t σ, R s ρ t σ.
-  
-  Global Instance allPrec : HasAll Prec :=
-    fun P => forall s ρ, P s ρ.
-  
-  Definition id : Relt :=
-    fun s ρ t σ => s = t /\ ρ = σ.
-  
-  Definition ptop : Prec :=
-    fun _ _ => True.
-  Definition rtop : Relt :=
-    fun _ _ _ _ => True.
+Global Instance stableRelt {E VE F} : HasStable (@Relt E VE F) :=
+  fun R Q => forall s ρ t σ, (R; Q ==> Q) s ρ t σ /\ (Q; R ==> Q) s ρ t σ.
 
-  Lemma stableRight {R Q : Relt} : Stable R Q -> All ((Q; R) ==> Q).
-  unfold Stable, stableRelt, All, allRelt.
-  intros.
-  specialize (H s ρ t σ).
-  destruct H.
-  easy.
-  Qed.
+Global Instance stablePrec {E VE F} : HasStable (@Prec E VE F) :=
+  fun R P => forall s ρ, ((fun t σ => exists s ρ, P s ρ /\ R s ρ t σ) ==> P) s ρ.
 
-  Lemma stableLeft {R Q : Relt} : Stable R Q -> All ((R; Q) ==> Q).
-  unfold Stable, stableRelt, All, allRelt.
-  intros.
-  specialize (H s ρ t σ).
-  destruct H.
-  easy.
-  Qed.
+Class HasAll A :=
+  All : A -> Prop.
 
-  Lemma precCompStable {R P Q} :
-    Stable R P ->
-    Stable R Q ->
-    Stable R (P;; Q).
-  intros.
-  unfold Stable, stablePrec, impl, implPrec.
-  intros.
-  do 6 destruct H1.
-  do 2 eexists.
-  split.
-  exact H1.
-  eapply stableRight.
-  easy.
-  do 2 eexists.
-  split.
-  exact H3.
-  easy.
-  Qed.
+Global Instance allRelt {E VE F} : HasAll (@Relt E VE F) :=
+  fun R => forall s ρ t σ, R s ρ t σ.
 
-  Lemma reltCompStable {R Q S : Relt} :
-    Stable R Q ->
-    Stable R S ->
-    Stable R (Q; S).
-  intros.
-  unfold Stable, stableRelt, impl, implRelt.
-  intros.
-  split.
-  intros.
-  do 3 destruct H1.
-  do 3 destruct H2.
-  do 2 eexists.
-  split.
-  eapply stableLeft.
-  easy.
-  do 2 eexists.
-  split.
-  exact H1.
-  exact H2.
-  easy.
-  intros.
-  do 6 destruct H1.
-  do 2 eexists.
-  split.
-  exact H1.
-  eapply stableRight.
-  easy.
-  do 2 eexists.
-  split.
-  exact H3.
-  easy.
-  Qed.
+Global Instance allPrec {E VE F} : HasAll (@Prec E VE F) :=
+  fun P => forall s ρ, P s ρ.
 
-  Lemma rtpStable {R Q : Relt} :
-    Stable R Q ->
-    Stable R (rtp Q).
-  intros.
-  unfold Stable, stablePrec, impl, implPrec, rtp.
-  intros.
-  do 5 destruct H0.
-  do 2 eexists.
-  eapply stableRight.
-  easy.
-  do 2 eexists.
-  split.
-  exact H0.
-  easy.
-  Qed.
+Definition id {E VE F} : @Relt E VE F :=
+  fun s ρ t σ => s = t /\ ρ = σ.
 
-End Predicates.
+Definition ptop {E VE F} : @Prec E VE F :=
+  fun _ _ => True.
+Definition rtop {E VE F} : @Relt E VE F :=
+  fun _ _ _ _ => True.
 
-Module Logic(O : OBJECT).
-  Module Ps := Predicates(O).
-  Import Ps.
-  Import O.
+Lemma stableRight {E VE F} {R Q : @Relt E VE F} : Stable R Q -> All ((Q; R) ==> Q).
+unfold Stable, stableRelt, All, allRelt.
+intros.
+specialize (H s ρ t σ).
+destruct H.
+easy.
+Qed.
 
-  Notation "ρ --> σ" := (exists t, AllRetEv t /\ LinRw (ρ ++ t) σ)
-    (at level 20).
+Lemma stableLeft {E VE F} {R Q : @Relt E VE F} : Stable R Q -> All ((R; Q) ==> Q).
+unfold Stable, stableRelt, All, allRelt.
+intros.
+specialize (H s ρ t σ).
+destruct H.
+easy.
+Qed.
 
-  Definition Commit i (impl : Impl E F)
-    (R G : Relt)
-    (P : Prec)
-    (ev : @Event E)
-    (Q : Relt) :=
-    forall s ρ t,
-    LinToSpec ρ VF ->
-    P s ρ ->
-    InterStep (impl:=impl) i s (i, liftUEv ev) t ->
-      exists σ,
-        Q s ρ t σ /\
-        G s ρ t σ /\
-        ρ --> σ.
-  
-  Definition VerifyPrim i (impl : Impl E F)
-    (R G : Relt)
-    (P : Prec)
-    (ev : @Event E)
-    (Q : Relt) :=
-    Stable R P /\
-    Stable R Q /\
-    Commit i impl R G P ev Q.
+Lemma precCompStable {E VE F} {R : @Relt E VE F} {P Q} :
+  Stable R P ->
+  Stable R Q ->
+  Stable R (P;; Q).
+intros.
+unfold Stable, stablePrec, impl, implPrec.
+intros.
+do 6 destruct H1.
+do 2 eexists.
+split.
+exact H1.
+eapply stableRight.
+easy.
+do 2 eexists.
+split.
+exact H3.
+easy.
+Qed.
 
-  CoInductive VerifyProg i (impl : Impl E F) : Relt -> Relt -> forall (A: Type), Prec -> Prog E A -> Relt -> Prop :=
-  | SafeReturn A v :
-      VerifyProg i impl rtop id A ptop (Return v) id
-  | SafeBind A B R G (P : Prec) (QI QR S : Relt) (m : E A) (k : A -> Prog E B) :
-      VerifyPrim i impl R G P (CallEv m) QI ->
-      (forall v,
-        VerifyPrim i impl R G (P;; QI) (RetEv m v) QR /\
-        VerifyProg i impl R G B (P;; QI;; QR) (k v) S) ->
-      VerifyProg i impl R G B P (Bind m k) (QI; QR; S)
-  | SafeNoOp A R G P C Q :
-      VerifyProg i impl R G A P C Q ->
-      VerifyProg i impl R G A P (NoOp C) Q
-  | SafeWeaken {A} {C : Prog E A} R R' G G' P P' Q Q' :
-      VerifyProg i impl R G A P C Q ->
-      Stable R' P' ->
-      Stable R' Q' ->
-      All (P' ==> P) ->
-      All (R' ==> R) ->
-      All (G ==> G') ->
-      All (Q ==> Q') ->
-      VerifyProg i impl R' G' A P' C Q'
-  .
-  Arguments VerifyProg i impl R G {A} P C Q.
+Lemma reltCompStable {E VE F} {R : @Relt E VE F} {Q S} :
+  Stable R Q ->
+  Stable R S ->
+  Stable R (Q; S).
+intros.
+unfold Stable, stableRelt, impl, implRelt.
+intros.
+split.
+intros.
+do 3 destruct H1.
+do 3 destruct H2.
+do 2 eexists.
+split.
+eapply stableLeft.
+easy.
+do 2 eexists.
+split.
+exact H1.
+exact H2.
+easy.
+intros.
+do 6 destruct H1.
+do 2 eexists.
+split.
+exact H1.
+eapply stableRight.
+easy.
+do 2 eexists.
+split.
+exact H3.
+easy.
+Qed.
 
-  Lemma SafeWeakenPost {i impl A} {C : Prog E A} R G P Q Q' :
-    VerifyProg i impl R G P C Q ->
-    Stable R Q' ->
-    VerifyProg i impl R G P C Q'.
-  Admitted.
+Notation "ρ --> σ" := (exists t, AllRetEv t /\ LinRw (ρ ++ t) σ)
+  (at level 20).
 
-  Definition TIdle (i : ThreadName) : Prec :=
-    fun s ρ =>
-      fst s i = Idle /\
-      true = even (length (@projAgent (@LEvent E F) i (map (fun e => (fst e, liftOEv (snd e))) ρ))).
+Definition Commit {E VE F} VF i (impl : Impl E F)
+  (R G : @Relt E VE F)
+  (P : @Prec E VE F)
+  (ev : @Event E)
+  (Q : @Relt E VE F) :=
+  forall s ρ t,
+  LinToSpec ρ VF ->
+  P s ρ ->
+  InterStep (impl:=impl) i s (i, liftUEv ev) t ->
+    exists σ,
+      Q s ρ t σ /\
+      G s ρ t σ /\
+      ρ --> σ.
 
-  Definition Invoke impl (i : ThreadName) Ret (m : F Ret) : Relt :=
-    fun s ρ t σ =>
-      TIdle i s ρ /\
-      σ = app ρ (cons (i, CallEv m) nil) /\
-      InterStep (impl:=impl) i s (i, OCallEv m) t.
-  
-  Inductive ReltRTC {R : Relt} : Relt :=
-  | Refl s ρ : ReltRTC s ρ s ρ
-  | Step s ρ t σ : R s ρ t σ -> ReltRTC s ρ t σ
-  | Trans s ρ t σ r τ :
-      ReltRTC s ρ t σ ->
-      ReltRTC t σ r τ ->
-      ReltRTC s ρ r τ.
-  Arguments ReltRTC : clear implicits.
+Definition VerifyPrim {E VE F} VF i (impl : Impl E F)
+  (R G : @Relt E VE F)
+  (P : @Prec E VE F)
+  (ev : @Event E)
+  (Q : @Relt E VE F) :=
+  Stable R P /\
+  Stable R Q /\
+  Commit VF i impl R G P ev Q.
 
-  Definition InvokeAny impl : Relt :=
-    fun s ρ t σ => exists i Ret (m : F Ret), Invoke impl i Ret m s ρ t σ.
+CoInductive VerifyProg {E VE F} VF i (impl : Impl E F) : @Relt E VE F -> @Relt E VE F -> forall (A: Type), @Prec E VE F -> Prog E A -> @Relt E VE F -> Prop :=
+| SafeReturn A v :
+    VerifyProg VF i impl rtop id A ptop (Return v) id
+| SafeBind A B R G P QI QR S (m : E A) (k : A -> Prog E B) :
+    VerifyPrim VF i impl R G P (CallEv m) QI ->
+    (forall v,
+      VerifyPrim VF i impl R G (P;; QI) (RetEv m v) QR /\
+      VerifyProg VF i impl R G B (P;; QI;; QR) (k v) S) ->
+    VerifyProg VF i impl R G B P (Bind m k) (QI; QR; S)
+| SafeNoOp A R G P C Q :
+    VerifyProg VF i impl R G A P C Q ->
+    VerifyProg VF i impl R G A P (NoOp C) Q
+| SafeWeaken {A} {C : Prog E A} R R' G G' P P' Q Q' :
+    VerifyProg VF i impl R G A P C Q ->
+    Stable R' P' ->
+    Stable R' Q' ->
+    All (P' ==> P) ->
+    All (R' ==> R) ->
+    All (G ==> G') ->
+    All (Q ==> Q') ->
+    VerifyProg VF i impl R' G' A P' C Q'
+.
+Arguments VerifyProg {E VE F} VF i impl R G {A} P C Q.
 
-  Definition InvokeMany impl :=
-    ReltRTC (InvokeAny impl).
+Definition TIdle {E VE F} (i : ThreadName) : @Prec E VE F :=
+  fun s ρ =>
+    fst s i = Idle /\
+    true = even (length (@projAgent (@LEvent E F) i (map (fun e => (fst e, liftOEv (snd e))) ρ))).
 
-  Definition Returned (i : ThreadName) {Ret} (m : F Ret) : Relt :=
-    fun s ρ t σ =>
-      s = t /\ ρ = σ /\
-      exists (v : Ret), 
-        fst t i = Cont m (Return v) /\
-        exists r,
-          projAgent i σ = app r (cons (i, RetEv m v) nil).
+Definition Invoke {E VE F} impl (i : ThreadName) Ret (m : F Ret) : @Relt E VE F :=
+  fun s ρ t σ =>
+    TIdle i s ρ /\
+    σ = app ρ (cons (i, CallEv m) nil) /\
+    InterStep (impl:=impl) i s (i, OCallEv m) t.
 
-  Definition Return (impl : Impl E F) (i : ThreadName) {Ret} (m : F Ret) : Relt :=
-    fun s ρ t σ =>
-      fst t i = Idle /\
-      σ = ρ /\
-      exists (v : Ret) r,
-        projAgent i σ = app r (cons (i, RetEv m v) nil) /\
-        InterStep (impl:=impl) i s (i, ORetEv m v) t.
+Inductive ReltRTC {E VE F} {R : @Relt E VE F} : @Relt E VE F :=
+| Refl s ρ : ReltRTC s ρ s ρ
+| Step s ρ t σ : R s ρ t σ -> ReltRTC s ρ t σ
+| Trans s ρ t σ r τ :
+    ReltRTC s ρ t σ ->
+    ReltRTC t σ r τ ->
+    ReltRTC s ρ r τ.
+Arguments ReltRTC {E VE F} R.
 
-  Definition ReturnAny impl : Relt :=
-    fun s ρ t σ => exists i Ret (m : F Ret), Return impl i m s ρ t σ.
+Definition InvokeAny {E VE F} impl : @Relt E VE F :=
+  fun s ρ t σ => exists i Ret (m : F Ret), Invoke impl i Ret m s ρ t σ.
 
-  Definition ReturnMany impl :=
-    ReltRTC (ReturnAny impl).
+Definition InvokeMany {E VE F} impl :=
+  ReltRTC (@InvokeAny E VE F impl).
 
-  Definition VerifyImpl
-    (R G : ThreadName -> Relt)
-    (P : ThreadName -> forall Ret, F Ret -> Prec)
-    (impl : Impl E F)
-    (Q : ThreadName -> forall Ret, F Ret -> Relt) : Prop :=
-    (forall i Ret (m : F Ret),
-      VerifyProg i impl (R i) (G i)
-        (P i Ret m;; Invoke impl i Ret m)
-        (impl Ret m)
-        (Q i Ret m; Returned i m)) /\
-    (forall i Ret (m : F Ret),
-      P i Ret m (allIdle, VE.(Init)) nil /\
-      All (P i Ret m ==> TIdle i) /\
-      Stable (R i) (P i Ret m) /\
-      Stable (R i) (Q i Ret m)) /\
-    (forall i, All (G i ==> R i)) /\
-    (forall i Ret1 (m1 : F Ret1) Ret2 (m2 : F Ret2),
-      All (P i Ret1 m1;; Invoke impl i Ret1 m1;; Q i Ret1 m1;; Returned i m1;; Return impl i m1 ==> P i Ret2 m2)).
-  
-  (* Theorem soundness (lay : Layer E F) :
-    (exists R G P Q, VerifyImpl R G P lay.(LImpl) Q) ->
-    specRefines VF (overObj lay).
-  intros.
-  destruct H as [R].
-  destruct H as [G].
-  destruct H as [P].
-  destruct H as [Q].
-  unfold VerifyImpl, specRefines, TransUtil.Incl in *.
-  destruct H.
-  destruct H0.
-  intros.
-  unfold IsTraceOfSpec, TransUtil.IsPathOf, TransUtil.Steps in *.
-  destruct H2 as [st].
-  Admitted. *)
-End Logic.
+Definition Returned {E VE F} (i : ThreadName) {Ret} (m : F Ret) : @Relt E VE F :=
+  fun s ρ t σ =>
+    s = t /\ ρ = σ /\
+    exists (v : Ret), 
+      fst t i = Cont m (Return v) /\
+      exists r,
+        projAgent i σ = app r (cons (i, RetEv m v) nil).
+
+Definition Return {E VE F} (impl : Impl E F) (i : ThreadName) {Ret} (m : F Ret) : @Relt E VE F :=
+  fun s ρ t σ =>
+    fst t i = Idle /\
+    σ = ρ /\
+    exists (v : Ret) r,
+      projAgent i σ = app r (cons (i, RetEv m v) nil) /\
+      InterStep (impl:=impl) i s (i, ORetEv m v) t.
+
+Definition ReturnAny {E VE F} impl : @Relt E VE F :=
+  fun s ρ t σ => exists i Ret (m : F Ret), Return impl i m s ρ t σ.
+
+Definition ReturnMany {E VE F} impl :=
+  ReltRTC (@ReturnAny E VE F impl).
+
+Definition VerifyImpl
+  {E F}
+  (VE : Spec E)
+  (VF : Spec F)
+  (R G : ThreadName -> @Relt E VE F)
+  (P : ThreadName -> forall Ret, F Ret -> @Prec E VE F)
+  (impl : Impl E F)
+  (Q : ThreadName -> forall Ret, F Ret -> @Relt E VE F) : Prop :=
+  (forall i Ret (m : F Ret),
+    VerifyProg VF i impl (R i) (G i)
+      (P i Ret m;; Invoke impl i Ret m)
+      (impl Ret m)
+      (Q i Ret m; Returned i m)) /\
+  (forall i Ret (m : F Ret),
+    P i Ret m (allIdle, VE.(Init)) nil /\
+    All (P i Ret m ==> TIdle i) /\
+    Stable (R i) (P i Ret m) /\
+    Stable (R i) (Q i Ret m)) /\
+  (forall i, All (G i ==> R i)) /\
+  (forall i Ret1 (m1 : F Ret1) Ret2 (m2 : F Ret2),
+    All (P i Ret1 m1;; Invoke impl i Ret1 m1;; Q i Ret1 m1;; Returned i m1;; Return impl i m1 ==> P i Ret2 m2)).
+
+(* Theorem soundness (lay : Layer E F) :
+  (exists R G P Q, VerifyImpl R G P lay.(LImpl) Q) ->
+  specRefines VF (overObj lay).
+intros.
+destruct H as [R].
+destruct H as [G].
+destruct H as [P].
+destruct H as [Q].
+unfold VerifyImpl, specRefines, TransUtil.Incl in *.
+destruct H.
+destruct H0.
+intros.
+unfold IsTraceOfSpec, TransUtil.IsPathOf, TransUtil.Steps in *.
+destruct H2 as [st].
+Admitted. *)
